PiLL/Model/STypes/Lemmas.lean
@@ -16,7 +16,7 @@ lemma Types.lc_dual {n : Nat} {A : Types} :
   A.lc n ↔  Aᗮ.lc n :=
   by induction A generalizing n <;> simp_all [Types.lc, Types.dual]
 
--- (A ↑ᵗ d, c).lc (n + c + d) ↔ A.lc (n + d)
+-- (A ↑ d, c).lc (n + c + d) ↔ A.lc (n + d)
 lemma Types.lc_shift_c_inv {n d c : Nat} {A : Types} :
   (A.shift d c).lc (n + c + d) ↔ A.lc (n + d) := by
   induction A generalizing n d c <;> simp_all only [Types.shift, Types.lc]
@@ -32,13 +32,13 @@ lemma Types.lc_mono {n : Nat} {A : Types} :
   intro hlc
   exact Types.lc_le (n := 0) (m := n) (by simp) hlc
 
--- A.lc n → (A ↑ᵗ d, c).lc (n + c)
+-- A.lc n → (A ↑ d, c).lc (n + c)
 lemma Types.lc_shift {n d c : Nat} {A : Types} :
   A.lc n → (A.shift d c).lc (n + c) := by
   induction A generalizing n d c <;>
     simp_all [Types.shift, TVar.shift, Types.lc, TVar.lc] <;> grind
 
--- A.lc n → (A ↑ᵗ 0, 1).lc (n + 1)
+-- A.lc n → (A ↑ 0, 1).lc (n + 1)
 lemma Types.lc_shift_0 {n : Nat} {A : Types} :
   A.lc n → (A.shift 0 1).lc (n + 1) := by
   intro h ; apply Types.lc_shift h
@@ -55,34 +55,34 @@ lemma Types.lc_subst_inv_0 {n : Nat} {A B : Types} (hA : A.lc n) :
   ((B.subst A 0).lc n ↔ B.lc (n + 1)) := by
   exact Types.lc_subst_inv (k := 0) hA
 
--- (A ↑ᵗ d, 1).lc (n + d + 1) ↔ A.lc (n + d)
+-- (A ↑ d, 1).lc (n + d + 1) ↔ A.lc (n + d)
 lemma Types.lc_shift_inv {n d : Nat} {A : Types} :
   (A.shift d 1).lc (n + d + 1) ↔ A.lc (n + d) := by
   induction A generalizing n d <;> simp_all only [Types.lc, Types.shift]
   case var v | varDual v => cases v <;> grind [TVar.shift, TVar.lc]
   case forall_ ihA | exists_ ihA => exact ihA (d := d + 1)
 
--- A⁺ᵗ.lc (n + 1) ↔ A.lc n
+-- A⁺.lc (n + 1) ↔ A.lc n
 lemma Types.lc_shift_inv_0 {n : Nat} {A : Types} :
   (A.shift 0 1).lc (n + 1) ↔ A.lc n := Types.lc_shift_inv (d := 0)
 
--- (A ↑ᵗ d, m) ↑ᵗ d, n = (A ↑ᵗ d, n) ↑ᵗ d, m
+-- (A ↑ d, m) ↑ d, n = (A ↑ d, n) ↑ d, m
 lemma Types.lc_shift_comm {A : Types} {d m n : Nat} :
   (A.shift d m).shift d n = (A.shift d n).shift d m := by
   induction A generalizing d m n <;> simp [Types.shift] <;> simp_all [TVar.shift] <;> grind
 
--- A⁺ᵗ ↑ᵗ k = (A ↑ᵗ k)⁺ᵗ
+-- A⁺ ↑ k = (A ↑ k)⁺
 lemma Types.lc_shift_comm_0 {A : Types} {k : Nat} :
   (A.shift 0 1).shift 0 k = (A.shift 0 k).shift 0 1 := Types.lc_shift_comm (d := 0)
 
--- (A ↑ᵗ d, a) ↑ᵗ d, b = A ↑ᵗ d, (a + b)
+-- (A ↑ d, a) ↑ d, b = A ↑ d, (a + b)
 lemma Types.shift_add {A : Types} {d a b : Nat} :
   (A.shift d a).shift d b = A.shift d (a + b) := by
   induction A generalizing d a b <;>
     simp_all only [Types.shift, var.injEq, varDual.injEq, TVar.shift]
   case var v | varDual v => cases v <;> grind
 
--- (A ↑ᵗ d, a) ↑ᵗ (d + a), b = A ↑ᵗ d, (a + b)
+-- (A ↑ d, a) ↑ (d + a), b = A ↑ d, (a + b)
 lemma Types.shift_accum {A : Types} {d a b : Nat} :
   (A.shift d a).shift (d + a) b = A.shift d (a + b) := by
   induction A generalizing d a b <;> simp [Types.shift, TVar.shift] <;> try grind
@@ -93,17 +93,17 @@ lemma Types.shift_accum_0 {A : Types} {a b : Nat} :
   have := Types.shift_accum (d := 0) (a := a) (b := b) (A := A)
   simp_all
 
--- (Aᗮ ↑ᵗ d, c) = (A ↑ᵗ d, c)ᗮ
+-- (Aᗮ ↑ d, c) = (A ↑ d, c)ᗮ
 lemma Types.shift_dual_comm {A : Types} {d c : Nat} :
   ((A.dual).shift d c) = (A.shift d c).dual := by
   induction A generalizing d c <;> simp_all [Types.shift, Types.dual, TVar.shift]
 
 lemma Types.shift_dual_comm_notation {A : Types} {d c : Nat} :
-  (Aᗮ ↑ᵗ d, c) = (A ↑ᵗ d, c)ᗮ := by
+  (Aᗮ ↑ d, c) = (A ↑ d, c)ᗮ := by
   induction A generalizing d c <;>
-    simp_all [HasShiftTypes.shift, Types.shift, Types.dual, TVar.shift]
+    simp_all [HasShift.shift, Types.shift, Types.dual, TVar.shift]
 
---  (A ↑ᵗ i, 1) ↑ᵗ (d + 1 + i), c = (A ↑ᵗ (d + i), c) ↑ᵗ i, 1
+--  (A ↑ i, 1) ↑ (d + 1 + i), c = (A ↑ (d + i), c) ↑ i, 1
 lemma Types.shift_comm {A : Types} {d c i : Nat} :
   (A.shift i 1).shift (d + 1 + i) c = (A.shift (d + i) c).shift i 1 := by
   induction A generalizing d c i <;>
@@ -111,11 +111,11 @@ lemma Types.shift_comm {A : Types} {d c i : Nat} :
   case var v | varDual v => cases v <;> grind
   case forall_ ih | exists_ ih => exact ih (d := d) (c := c) (i := i + 1)
 
--- (A ↑ᵗ 1) ↑ᵗ (d + 1), c = (A.↑ᵗ d, c) ↑ᵗ 1
+-- (A ↑ 1) ↑ (d + 1), c = (A.↑ d, c) ↑ 1
 lemma Types.shift_comm_0 {A : Types} {d c : Nat} :
  (A.shift 0 1).shift (d + 1) c = (A.shift d c).shift 0 1 := Types.shift_comm (i := 0)
 
--- (B{A // k}) ↑ᵗ d, c = (B ↑ᵗ (d + 1), c){(A ↑ᵗ d, c) // k}
+-- (B{A // k}) ↑ d, c = (B ↑ (d + 1), c){(A ↑ d, c) // k}
 lemma Types.shift_subst_comm_depth_ge_idx {A B : Types} {d c i : Nat} (hle : i ≤ d) :
   (B.subst A i).shift d c = (B.shift (d + 1) c).subst (A.shift d c) i := by
   induction B generalizing d c i A <;> simp only [Types.shift, Types.subst] <;>
@@ -128,12 +128,12 @@ lemma Types.shift_subst_comm_depth_ge_idx {A B : Types} {d c i : Nat} (hle : i �
     | free => rfl
   case forall_ B ih | exists_ => grind [Types.shift_comm_0]
 
--- (B{A // 0}) ↑ᵗ d, c = (B ↑ᵗ (d + 1), c){(A ↑ᵗ d, c) // 0}
+-- (B{A // 0}) ↑ d, c = (B ↑ (d + 1), c){(A ↑ d, c) // 0}
 lemma Types.shift_subst_0_comm {A B : Types} {d c : Nat} :
   (B.subst A 0).shift d c = (B.shift (d + 1) c).subst (A.shift d c) 0 :=
   Types.shift_subst_comm_depth_ge_idx (by simp)
 
--- B{A // i} ↑ᵗ d, c = (B ↑ᵗ d, c){(A ↑ᵗ d, c) // (i + c)}
+-- B{A // i} ↑ d, c = (B ↑ d, c){(A ↑ d, c) // (i + c)}
 lemma Types.shift_subst_comm_depth_le_idx {A B : Types} {d c i : Nat} (hle : d ≤ i) :
   (B.subst A i).shift d c = (B.shift d c).subst (A.shift d c) (i + c) := by
   induction B generalizing A d c i <;>
@@ -146,14 +146,14 @@ lemma Types.shift_subst_comm_depth_le_idx {A B : Types} {d c i : Nat} (hle : d �
     | free => rfl
   case forall_ ih | exists_ ih => grind [Types.shift_comm_0]
 
--- B{A // i} ↑ᵗ c = (B ↑ᵗ c){(A ↑ᵗ c) // (i + c)}
+-- B{A // i} ↑ c = (B ↑ c){(A ↑ c) // (i + c)}
 lemma Types.shift_0_subst_comm {A B : Types} {c i : Nat} :
   (B.subst A i).shift 0 c = (B.shift 0 c).subst (A.shift 0 c) (i + c) :=
   Types.shift_subst_comm_depth_le_idx (by simp)
 
 @[simp] lemma Types.isServerUsable_shift {d c : Nat} {A : Types} :
-  A.isServerUsable ↔ (A ↑ᵗ d, c).isServerUsable := by
-  cases A <;> simp [HasShiftTypes.shift, Types.shift, Types.isServerUsable]
+  A.isServerUsable ↔ (A ↑ d, c).isServerUsable := by
+  cases A <;> simp [HasShift.shift, Types.shift, Types.isServerUsable]
 
 lemma Types.lc_subst_lc_eq_lc_gen {A B : Types} {n n' k : Nat} :
   n' ≤ n → k ≤ n → Types.lc n B → Types.lc n' A → Types.lc n (B.subst A k) := by
@@ -188,9 +188,9 @@ lemma Types.subst_dual_comm {A B : Types} {k : Nat} :
   case var v | varDual v => cases v <;> grind [TVar.shift, Types.subst]
 
 @[simp] lemma Types.shiftTypes_substTypes_cancel_0 {A B : Types} :
-  B⁺ᵗ{A // 0} = B := Types.shift_subst_cancel (A := B) (B := A) (d := 0)
+  B⁺{A // 0} = B := Types.shift_subst_cancel (A := B) (B := A) (d := 0)
 
--- B{A' // d}{A // i} = B{A ↑ᵗ d, 1 // i + 1}{A'{A // i} // d}
+-- B{A' // d}{A // i} = B{A ↑ d, 1 // i + 1}{A'{A // i} // d}
 lemma Types.subst_comm {A A' B : Types} {d i : Nat} (hle : d ≤ i) :
   (B.subst A' d).subst A i = (B.subst (A.shift d 1) (i + 1)).subst (A'.subst A i) d := by
   induction B generalizing A A' d i hle <;>
@@ -204,7 +204,7 @@ lemma Types.subst_comm {A A' B : Types} {d i : Nat} (hle : d ≤ i) :
       )
     )
 
-  -- B{A' // 0}{A // k} = B{A ↑ᵗ 0, 1 // k + 1}{A'{A // k} // 0}
+  -- B{A' // 0}{A // k} = B{A ↑ 0, 1 // k + 1}{A'{A // k} // 0}
 lemma Types.subst_comm_0 {A A' B : Types} {i : Nat} :
   (B.subst A' 0).subst A i = (B.subst (A.shift 0 1) (i + 1)).subst (A'.subst A i) 0 :=
     Types.subst_comm (by simp)
